@@ -352,3 +352,6 @@ import Xv6.LinkConsoleinit
 import Xv6.ProofUartwrite
 import Xv6.LinkUartwrite
 import Xv6.ProofUartintr
+import Xv6.ProofConsoleintr
+import Xv6.LinkConsoleintr
+import Xv6.LinkUartintr
